More work in progress on reflective indexed splitter

src/Parsers/Refinement/IndexedAndAtMostOneNonTerminalReflective.v
@@ -1,14 +1,28 @@
-(** * Reflective helpers for simply-typed interface of the parser *)
-Require Import Coq.Lists.List Coq.Strings.String.
-Require Import ADTSynthesis.Parsers.ContextFreeGrammar.
-Require Import ADTSynthesis.Parsers.ContextFreeGrammarProperties.
-Require Import ADTSynthesis.Parsers.ContextFreeGrammarEquality.
+(** First step of a splitter refinement; indexed representation, and handle all rules with at most one nonterminal; leave a reflective goal *)
+Require Import Coq.Strings.String Coq.Arith.Lt Coq.Lists.List.
+Require Import Coq.Numbers.Natural.Peano.NPeano.
+Require Import ADTSynthesis.Parsers.StringLike.Core.
 Require Import ADTSynthesis.Parsers.ParserInterface.
-Require Import ADTSynthesis.Parsers.Refinement.IndexedAndAtMostOneNonTerminal.
-Require Import ADTSynthesis.Computation.Core.
+Require Import ADTSynthesis.Parsers.ParserADTSpecification.
+Require Import ADTSynthesis.Parsers.StringLike.Properties.
+Require Import ADTSynthesis.Parsers.StringLike.String.
+Require Import ADTSynthesis.Parsers.ContextFreeGrammarEquality.
+Require Import ADTNotation.BuildADT ADTNotation.BuildADTSig.
+Require Import ADT.ComputationalADT.
 Require Import ADTSynthesis.Common ADTSynthesis.Common.Equality.
+Require Import ADTSynthesis.ADTRefinement.
+Require Import ADTSynthesis.Common.StringBound ADTSynthesis.Common.ilist.
+Require Import ADTRefinement.BuildADTRefinements.HoneRepresentation.
+Require Import ADTSynthesis.Common.IterateBoundedIndex.
+Require Import ADTSynthesis.Common.List.FlattenList.
+Require Import ADTSynthesis.Common.List.ListFacts.
 
 Set Implicit Arguments.
+
+Local Open Scope list_scope.
+Local Open Scope ADTSig_scope.
+Local Open Scope ADT_scope.
+Local Open Scope string_scope.
 
 Fixpoint tails {A} (ls : list A) : list (list A)
   := match ls with
@@ -22,8 +36,8 @@ Definition forall_reachable_productions {Char} (G : grammar Char) {T} (f : produ
   := fold_right
        f
        init
-       (flatten1
-          (flatten1
+       (flatten
+          (flatten
              (map
                 (fun nt =>
                    (map
@@ -31,16 +45,154 @@ Definition forall_reachable_productions {Char} (G : grammar Char) {T} (f : produ
                       (Lookup G nt)))
                 (Valid_nonterminals G)))).
 
-Global Arguments forall_reachable_productions / .
+Lemma exists_in_map_tails {A} (P : _ -> Prop) ls
+: (forall p : list A, (exists prefix, In (prefix ++ p)%list ls) -> P p)
+  <-> fold_right and True (map P (flatten (map tails ls))).
+Proof.
+  induction ls as [ | x xs ]; simpl; split; intros; eauto;
+  try solve [ eauto
+            | destruct_head ex; destruct_head False ].
+  { rewrite map_app, fold_right_app.
+    apply fold_right_and_iff; split.
+    { clear IHxs.
+      specialize (fun p prefix H' => H p (ex_intro _ prefix (or_introl H'))).
+      induction x; simpl; split; try tauto.
+      { apply (H _ []); reflexivity. }
+      { apply (H _ []); reflexivity. }
+      { apply IHx; intros p prefix H'; subst.
+        eapply (H _ (_::prefix)); reflexivity. } }
+    { apply IHxs; intros; destruct_head ex.
+      apply H; eexists; right; eassumption. } }
+  { repeat match goal with
+             | [ H : _ |- _ ] => rewrite map_app in H
+             | [ H : _ |- _ ] => rewrite fold_right_app in H
+             | [ H : fold_right _ ?init _ |- _ ] => not constr_eq init True; apply fold_right_and_iff in H
+             | _ => progress destruct_head_hnf and
+             | _ => progress destruct_head or
+             | _ => progress destruct_head ex
+             | _ => progress subst
+             | _ => progress eauto
+             | [ H : ?T, H' : ?T -> ?X |- _ ] => specialize (H' H)
+           end.
+    let H := match goal with H : fold_right and True (map P (tails (_ ++ ?p))) |- P ?p => constr:H end in
+    clear -H.
+    match goal with
+      | [ H : fold_right and True (map P (tails (?x ++ _))) |- P ?p ] => induction x; destruct p
+    end;
+      simpl in *;
+      destruct_head and; eauto. }
+Qed.
 
-Section interface.
+Lemma production_is_reachable__forall_reachable_productions {Char} {G : grammar Char} (P : production Char -> Prop)
+: (forall p, production_is_reachable G p -> P p)
+  <-> (forall_reachable_productions G (fun p H => P p /\ H) True).
+Proof.
+  unfold forall_reachable_productions, production_is_reachable.
+  pose proof (fold_right_map P and) as H; unfold compose in *; simpl in *.
+  rewrite <- H.
+  induction (Valid_nonterminals G) as [ | x xs IHG ]; simpl in *.
+  { split; simpl; intros; trivial.
+    destruct_head ex; destruct_head and; destruct_head False. }
+  { rewrite flatten_app, map_app, fold_right_app.
+    setoid_rewrite fold_right_and_iff.
+    setoid_rewrite <- exists_in_map_tails.
+    setoid_rewrite <- IHG; clear IHG.
+    repeat (split || intro); destruct_head ex; destruct_head and; destruct_head or; subst;
+    match goal with
+      | [ H : _ |- _ ] => apply H
+    end;
+    repeat match goal with
+             | [ |- ex _ ] => eexists
+             | _ => eassumption
+             | [ |- _ /\ _ ] => split; eassumption
+             | [ |- _ /\ _ ] => split; [ left; reflexivity | eassumption ]
+             | [ |- _ /\ _ ] => split; [ right; eassumption | eassumption ]
+           end. }
+Qed.
+
+Lemma production_is_reachable__forall_reachable_productions' {Char} {G : grammar Char} (P : _ -> _ -> Prop)
+: (forall p ps, production_is_reachable G (p::ps) -> P p ps)
+  <-> (forall_reachable_productions G (fun p H => match p with
+                                                    | nil => True
+                                                    | x::xs => P x xs
+                                                  end /\ H) True).
+Proof.
+  setoid_rewrite <- production_is_reachable__forall_reachable_productions.
+  split; intro H.
+  { intros []; intuition. }
+  { intros p ps.
+    specialize (H (p::ps)); eauto. }
+Qed.
+
+Section helpers.
+  Section generic.
+    Context {Char : Type}.
+
+    Fixpoint has_only_terminals (its : production Char)
+    : bool
+      := match its with
+           | nil => true
+           | (Terminal _)::xs => has_only_terminals xs
+           | (NonTerminal _)::_ => false
+         end.
+  End generic.
+
+  Section generic_string.
+    Context {Char} {HSL : StringLike Char} {HLSP : StringLikeProperties Char} (G : grammar Char).
+
+    Lemma has_only_terminals_length {its str}
+          (H0 : @has_only_terminals _ its)
+          (H1 : parse_of_production G str its)
+    : length str = List.length its.
+    Proof.
+      induction H1 as [ | ? ? ? ? pit pits IH ]; simpl in *; trivial.
+      rewrite drop_length in IH.
+      dependent destruction pit.
+      { match goal with
+          | [ H : context[(_ ~= [ _ ])%string_like] |- _ ]
+            => apply length_singleton in H
+        end.
+        rewrite <- IH by assumption; clear IH.
+        repeat match goal with
+                 | _ => intro
+                 | [ H : context[length (take _ _)] |- _ ] => rewrite take_length in H
+                 | [ H : context[length (drop _ _)] |- _ ] => rewrite drop_length in H
+                 | [ H : min ?x ?y = 1 |- _ ] => is_var x; destruct x
+                 | [ H : min (S ?x) ?y = 1 |- _ ] => is_var x; destruct x
+                 | [ H : min (S (S ?x)) ?y = 1 |- _ ] => revert H; apply (Min.min_case_strong (S (S x)) y)
+                 | [ H : context[min _ 0] |- _ ] => rewrite Min.min_0_r in H
+                 | [ H : context[min 0 _] |- _ ] => rewrite Min.min_0_l in H
+                 | [ H : 0 = 1 |- _ ] => exfalso; clear -H; discriminate
+                 | [ H : S (S _) = 1 |- _ ] => exfalso; clear -H; discriminate
+                 | [ H : ?x = 1, H' : context[?x] |- _ ] => rewrite H in H'
+                 | [ H : ?x = 1 |- context[?x] ] => rewrite H
+                 | [ H : min ?x ?y = 1 |- _ ] => revert H; apply (Min.min_case_strong x y)
+                 | _ => omega
+               end. }
+      { exfalso.
+        unfold is_true in *.
+        discriminate. }
+    Qed.
+  End generic_string.
+End helpers.
+
+Section IndexedImpl.
   Context (G : grammar Ascii.ascii).
 
+  Local Notation T := (String.string * (nat * nat))%type (only parsing).
+
+  Local Notation string_of_indexed s :=
+    (substring (fst (snd s)) (snd (snd s)) (fst s))
+      (only parsing).
+  Local Notation ilength s :=
+    (min (String.length (fst s) - fst (snd s)) (snd (snd s)))
+      (only parsing).
+
   Definition expanded_fallback_list
-             (s : (String.string * (nat * nat)))
+             (s : T)
              (it : item Ascii.ascii) (its : production Ascii.ascii)
              (dummy : list nat)
-  : Comp ((String.string * (nat * nat)) * list nat)
+  : Comp (T * list nat)
     := (ls <- (forall_reachable_productions
                  G
                  (fun p else_case
@@ -62,10 +214,755 @@ Section interface.
                                            -> List.In n splits }
                            end)
                      else else_case)
-                 (ret dummy));
+                 (ret (match its, it with
+                         | nil, _
+                           => [ilength s]
+                         | _::_, Terminal _
+                           => [1]
+                         | _::_, NonTerminal _
+                           => if has_only_terminals its
+                              then [ilength s - List.length its]
+                              else dummy
+                       end)));
         ret (s, ls))%comp.
 
   Global Arguments expanded_fallback_list / .
+
+
+  (** Reference implementation of a [String] that can be split; has a [string], and a start index, and a length *)
+
+  Definition rindexed_spec : ADT (string_rep Ascii.ascii) := ADTRep T {
+    Def Constructor "new"(s : String.string) : rep :=
+      ret (s, (0, String.length s)),
+
+    Def Method "to_string"(s : rep, x : unit) : String.string :=
+      ret (s, string_of_indexed s),
+
+    Def Method "is_char"(s : rep, ch : Ascii.ascii) : bool  :=
+      ret (s, string_beq (string_of_indexed s) (String.String ch "")),
+
+    Def Method "length"(s : rep, x : unit) : nat :=
+      ret (s, ilength s),
+
+    Def Method "take"(s : rep, n : nat) : unit :=
+      ret ((fst s, (fst (snd s), min (snd (snd s)) n)), tt),
+
+    Def Method "drop"(s : rep, n : nat) : unit :=
+      ret ((fst s, (fst (snd s) + n, snd (snd s) - n)), tt),
+
+    Def Method "splits"(s : rep, p : item Ascii.ascii * production Ascii.ascii) : list nat :=
+      dummy <- { ls : list nat | True };
+      expanded_fallback_list s (fst p) (snd p) dummy
+  }.
+
+  Local Ltac fin :=
+    repeat match goal with
+             | _ => progress unfold split_list_is_complete
+             | _ => progress simpl in *
+             | _ => progress computes_to_inv
+             | _ => progress subst
+             | [ |- computes_to (Bind _ _) _ ]
+               => refine ((fun H0 H1 => BindComputes _ _ _ _ H1 H0) _ _)
+             | [ |- computes_to (Return ?x) ?y ]
+               => cut (x = y);
+                 [ let H := fresh in intro H; try rewrite H; eapply ReturnComputes | ]
+             | [ |- computes_to (Pick _) _ ]
+               => eapply PickComputes
+             | _ => reflexivity
+             | _ => assumption
+           end;
+    try solve [ rewrite substring_correct3'; reflexivity
+              | repeat match goal with
+                         | _ => intro
+                         | _ => reflexivity
+                         | _ => rewrite substring_substring
+                         | _ => rewrite Nat.sub_0_r
+                         | _ => rewrite substring_length
+                         | _ => rewrite Nat.add_sub
+                         | _ => rewrite <- Nat.sub_min_distr_r
+                         | _ => progress simpl
+                         | [ |- context[min ?x ?y] ]
+                           => match goal with
+                                | [ |- context[min y x] ]
+                                  => rewrite (Min.min_comm x y)
+                              end
+                         | [ |- context[min (min _ ?x) (?x - ?y)] ]
+                           => rewrite <- (Min.min_assoc _ x (x - y)), (Min.min_r x (x - y)) by omega
+                         | [ |- substring (?x + ?y) _ _ = substring (?y + ?x) _ _ ]
+                           => rewrite (Plus.plus_comm x y)
+                         | [ |- substring ?x ?y ?z = substring ?x (min ?w ?y) ?z ]
+                           => apply (@Min.min_case_strong w y)
+                         | [ H : _ |- _ ] => rewrite Min.min_assoc in H
+                         | _ => apply substring_correct4; omega
+                       end
+              | repeat match goal with
+                         | _ => intro
+                         | _ => progress subst
+                         | [ |- List.In ?x [?y] ] => left
+                         | _ => reflexivity
+                         | [ H : parse_of_production _ _ nil |- _ ] => let H' := fresh in rename H into H'; dependent destruction H'
+                         | [ H : parse_of_production _ _ (_::_) |- _ ] => let H' := fresh in rename H into H'; dependent destruction H'
+                         | [ H : parse_of_item _ _ (Terminal _) |- _ ] => let H' := fresh in rename H into H'; dependent destruction H'
+                         | [ H : parse_of_item _ _ (NonTerminal _) |- _ ] => let H' := fresh in rename H into H'; dependent destruction H'
+                         | _ => erewrite <- has_only_terminals_length by eassumption
+                         | [ H : _ |- _ ] => progress rewrite ?(@drop_length _ string_stringlike string_stringlike_properties), ?(@take_length _ string_stringlike string_stringlike_properties), ?substring_length, ?Nat.add_sub, <- ?plus_n_O, ?Minus.minus_diag, ?Nat.sub_0_r, ?sub_plus in H by omega
+                         | _ => progress rewrite ?drop_length, ?take_length, ?substring_length, ?Nat.add_sub, ?Minus.minus_diag, ?Nat.sub_0_r, <- ?plus_n_O, ?sub_plus by omega
+                         | [ H : is_true (string_beq _ _) |- _ ] => apply string_bl in H
+                         | [ |- _ \/ False ] => left
+                         | [ H : substring _ _ _ = String.String _ _ |- _ = _ :> nat ] => apply (f_equal String.length) in H; simpl in H
+                         | [ H : context[(_ ~= [ _ ])%string_like] |- _ ]
+                           => apply length_singleton in H
+                         | [ |- context[min ?x (?y + ?z) - ?z] ]
+                           => rewrite <- (Nat.sub_min_distr_r x (y + z) z)
+                         | [ H : context[min ?x (?y + ?z) - ?z] |- _ ]
+                           => rewrite <- (Nat.sub_min_distr_r x (y + z) z) in H
+                         | [ H : min ?x ?y = 1 |- _ ] => is_var x; revert H; apply (Min.min_case_strong x y)
+                         | [ H : min ?x ?y = 1 |- _ ] => is_var y; revert H; apply (Min.min_case_strong x y)
+                         | [ H : min ?x ?y = 0 |- _ ] => is_var x; revert H; apply (Min.min_case_strong x y)
+                         | [ H : min ?x ?y = 0 |- _ ] => is_var y; revert H; apply (Min.min_case_strong x y)
+                         | [ H : min ?x 1 = 0 |- _ ] => revert H; apply (Min.min_case_strong x 1)
+                         | [ |- context[0 + ?x] ] => change (0 + x) with x
+                         | [ |- context[?x - S ?y] ]
+                           => not constr_eq y 0; rewrite !(Nat.sub_succ_r x y), !Minus.pred_of_minus
+                         | [ H : ?x = 1 |- context[?x] ] => rewrite H
+                         | [ H : ?x = 1, H' : context[?x] |- _ ] => rewrite H in H'
+                         | [ H : ?x <= ?y |- context[?x - ?y] ] => replace (x - y) with 0 by (clear -H; omega)
+                         | [ H : context[?x - ?y], H' : ?x <= ?y |- _ ]
+                           => rewrite (proj2 (@Nat.sub_0_le x y)) in H by exact H'
+                         | [ H : context[min 0 ?x] |- _ ] => change (min 0 x) with 0 in H
+                         | [ |- 1 = ?x ] => is_var x; destruct x
+                         | [ |- 1 = S ?x ] => is_var x; destruct x
+                         | [ H : _ <= 0 |- _ ] => apply Le.le_n_0_eq in H; symmetry in H
+                         | [ H : context[min 1 ?x] |- _ ] => is_var x; destruct x
+                         | [ H : context[min 1 (S ?x)] |- _ ] => is_var x; destruct x
+                         | [ H : context[min 1 (S ?x)] |- _ ] => change (min 1 (S x)) with 1 in H
+                         | [ H : context[min ?x ?y], H' : ?x <= ?y |- _ ] => rewrite Min.min_l in H by assumption
+                         | [ H : context[min ?x ?y], H' : ?y <= ?x |- _ ] => rewrite Min.min_r in H by assumption
+                         | [ H : context[min (?x - ?y) ?x] |- _ ] => rewrite Min.min_l in H by omega
+                         | [ H : context[min ?x (?x - ?y)] |- _ ] => rewrite Min.min_r in H by omega
+                         | _ => omega
+                       end ].
+
+  Local Ltac fin2 :=
+    repeat match goal with
+             | [ H : fold_right and _ (map _ ?ls) |- fold_right and _ (map _ ?ls) ]
+               => revert H; apply fold_right_and_map_impl
+             | _ => intro
+             | _ => progress subst
+             | [ H : false = true |- _ ] => exfalso; clear -H; discriminate
+             | [ H : context[if has_only_terminals ?ls then _ else _] |- _ ]
+               => revert H; case_eq (has_only_terminals ls)
+             | [ |- context[production_beq ?d ?x ?y] ]
+               => case_eq (production_beq d x y); intro
+             | [ H : context[if production_beq ?d ?x ?y then _ else _] |- _ ]
+               => revert H; case_eq (production_beq d x y); intro
+             | [ H : production_beq _ _ _ = true |- _ ] => apply (production_bl (@ascii_bl)) in H
+             | [ H : (_::_) = (_::_) |- _ ] => inversion H; clear H
+             | _ => progress eauto
+             | [ |- context[match ?x with _ => _ end] ] => atomic x; destruct x
+             | [ H : _ -> _ |- _ ] => clear H; solve [ fin ]
+           end.
+
+  Lemma FirstStep
+  : refineADT (string_spec G) rindexed_spec.
+  Proof.
+    econstructor 1 with (AbsR := (fun r_o r_n =>
+                                    substring (fst (snd r_n)) (snd (snd r_n)) (fst r_n) = r_o));
+
+        eapply Iterate_Ensemble_BoundedIndex_equiv;
+        simpl; intuition; intros; try simplify with monad laws;
+        repeat intro; computes_to_inv; subst; simpl;
+        fin.
+    { intros.
+      match goal with
+        | [ H : production_is_reachable G (?x::?xs) |- _ ]
+          => move H at top; generalize dependent xs; intros xs H; move H at top; generalize dependent x; intros x H; revert x xs H
+      end.
+      refine (proj2 (@production_is_reachable__forall_reachable_productions' Ascii.ascii G _) _).
+      unfold forall_reachable_productions.
+      lazymatch goal with
+        | [ |- context[fold_right (fun x y => @?P x /\ y) _ _] ]
+          => let H' := fresh in
+             pose proof (fold_right_map P and) as H';
+               unfold compose in H'; simpl in H';
+               rewrite <- H'; clear H'
+      end.
+      generalize (flatten
+                    (flatten
+                       (map (fun nt : string => map tails (G nt))
+                            (Valid_nonterminals G)))).
+      intro ls; induction ls; simpl; trivial; [].
+      { repeat match goal with
+                 | [ |- _ /\ _ ] => split
+                 | [ |- context[match ?e with _ => _ end] ] => atomic e; destruct e
+                 | [ |- context[production_beq _ ?x ?x] ] => rewrite (production_lb (@ascii_lb) eq_refl)
+                 | _ => solve [ trivial ]
+               end.
+        { clear IHls; intros; abstract fin. }
+        { clear IHls; intros; abstract fin. }
+        { clear IHls; intros; abstract fin. }
+        { admit. }
+        { abstract fin2. }
+        { abstract fin2. }
+        { abstract fin2. }
+        { fin2.
+          match goal with
+          end.
+          { fin2.
+            match goal with
+            end.
+            fin2.
+            clear H4.
+            destruct i; fin2; fin;
+            try match goal with
+                end.
+            left; fin.
+            pose has_only_terminals_length.
+            Focus 2.
+            { fin.
+            Local Opaque has_only_terminals.
+            fin.
+ }
+        { revert IHls; apply fold_right_and_map_impl; trivial; [].
+          intros []; trivial.
+          repeat match goal with
+                   | _ => intro
+                   | _ => progress subst
+                   | [ |- context[production_beq ?d ?x ?y] ]
+                     => case_eq (production_beq d x y); intro
+                   | [ H : context[if production_beq ?d ?x ?y then _ else _] |- _ ]
+                     => revert H; case_eq (production_beq d x y); intro
+                   | [ H : production_beq _ _ _ = true |- _ ] => apply (production_bl (@ascii_bl)) in H
+                   | [ H : (_::_) = (_::_) |- _ ] => inversion H; clear H
+                   | _ => progress eauto
+                   | [ H : _ -> _ |- _ ] => clear H; solve [ fin ]
+                 end. }
+        { revert IHls; apply fold_right_and_map_impl; trivial; [].
+          intros []; trivial.
+          repeat match goal with
+                   | _ => intro
+                   | _ => progress subst
+                   | [ |- context[production_beq ?d ?x ?y] ]
+                     => case_eq (production_beq d x y); intro
+                   | [ H : context[if production_beq ?d ?x ?y then _ else _] |- _ ]
+                     => revert H; case_eq (production_beq d x y); intro
+                   | [ H : production_beq _ _ _ = true |- _ ] => apply (production_bl (@ascii_bl)) in H
+                   | [ H : (_::_) = (_::_) |- _ ] => inversion H; clear H
+                   | _ => progress eauto
+                   | [ H : _ -> _ |- _ ] => clear H; solve [ fin ]
+                 end. }
+
+          { clear H1.
+
+fin.
+apply H1; eauto.
+
+
+                   | [ H : parse_of_production _ _ nil |- _ ] => let H' := fresh in rename H into H'; dependent destruction H'
+                   | [ H : parse_of_production _ _ (_::_) |- _ ] => let H' := fresh in rename H into H'; dependent destruction H'
+                   | [ H : parse_of_item _ _ (Terminal _) |- _ ] => let H' := fresh in rename H into H'; dependent destruction H'
+                   | [ H : parse_of_item _ _ (NonTerminal _) |- _ ] => let H' := fresh in rename H into H'; dependent destruction H'
+                   | _ => progress computes_to_inv
+                 end.
+          apply H1; eauto.
+          { intros; fin. }
+          { intros; fin.
+            eauto. } }
+{
+ fin.
+intros.
+
+  intuition.
+  intros init1 init2 H.
+ SearchAbout fold_right.
+clear IHls; intros; fin.
+repeat match goal with
+                         | _ => intro
+                         | _ => progress subst
+                         | [ |- List.In ?x [?y] ] => left
+                         | _ => reflexivity
+                         | [ H : parse_of_production _ _ nil |- _ ] => let H' := fresh in rename H into H'; dependent destruction H'
+                         | [ H : parse_of_production _ _ (_::_) |- _ ] => let H' := fresh in rename H into H'; dependent destruction H'
+                         | [ H : parse_of_item _ _ (Terminal _) |- _ ] => let H' := fresh in rename H into H'; dependent destruction H'
+                         | [ H : parse_of_item _ _ (NonTerminal _) |- _ ] => let H' := fresh in rename H into H'; dependent destruction H'
+                         | _ => erewrite <- has_only_terminals_length by eassumption
+                         | [ H : _ |- _ ] => progress rewrite ?(@drop_length _ string_stringlike string_stringlike_properties), ?(@take_length _ string_stringlike string_stringlike_properties), ?substring_length, ?Nat.add_sub, <- ?plus_n_O, ?Minus.minus_diag, ?Nat.sub_0_r, ?sub_plus in H by omega
+                         | _ => progress rewrite ?drop_length, ?take_length, ?substring_length, ?Nat.add_sub, ?Minus.minus_diag, ?Nat.sub_0_r, <- ?plus_n_O, ?sub_plus by omega
+                         | [ H : is_true (string_beq _ _) |- _ ] => apply string_bl in H
+                         | [ |- _ \/ False ] => left
+                         | [ H : substring _ _ _ = String.String _ _ |- _ = _ :> nat ] => apply (f_equal String.length) in H; simpl in H
+                         | [ H : context[(_ ~= [ _ ])%string_like] |- _ ]
+                           => apply length_singleton in H
+                         | [ |- context[min ?x (?y + ?z) - ?z] ]
+                           => rewrite <- (Nat.sub_min_distr_r x (y + z) z)
+                         | [ H : context[min ?x (?y + ?z) - ?z] |- _ ]
+                           => rewrite <- (Nat.sub_min_distr_r x (y + z) z) in H
+                         | [ H : min ?x ?y = 1 |- _ ] => is_var x; revert H; apply (Min.min_case_strong x y)
+                         | [ H : min ?x ?y = 1 |- _ ] => is_var y; revert H; apply (Min.min_case_strong x y)
+                         | [ H : min ?x ?y = 0 |- _ ] => is_var x; revert H; apply (Min.min_case_strong x y)
+                         | [ H : min ?x ?y = 0 |- _ ] => is_var y; revert H; apply (Min.min_case_strong x y)
+                         | [ H : min ?x 1 = 0 |- _ ] => revert H; apply (Min.min_case_strong x 1)
+                         | [ |- context[0 + ?x] ] => change (0 + x) with x
+                         | [ |- context[?x - S ?y] ]
+                           => not constr_eq y 0; rewrite !(Nat.sub_succ_r x y), !Minus.pred_of_minus
+                         | [ H : ?x = 1 |- context[?x] ] => rewrite H
+                         | [ H : ?x = 1, H' : context[?x] |- _ ] => rewrite H in H'
+                         | [ H : ?x <= ?y |- context[?x - ?y] ] => replace (x - y) with 0 by (clear -H; omega)
+                         | [ H : context[?x - ?y], H' : ?x <= ?y |- _ ]
+                           => rewrite (proj2 (@Nat.sub_0_le x y)) in H by exact H'
+                         | [ H : context[min 0 ?x] |- _ ] => change (min 0 x) with 0 in H
+                         | [ |- 1 = ?x ] => is_var x; destruct x
+                         | [ |- 1 = S ?x ] => is_var x; destruct x
+                         | [ H : _ <= 0 |- _ ] => apply Le.le_n_0_eq in H; symmetry in H
+                         | [ H : context[min 1 ?x] |- _ ] => is_var x; destruct x
+                         | [ H : context[min 1 (S ?x)] |- _ ] => is_var x; destruct x
+                         | [ H : context[min 1 (S ?x)] |- _ ] => change (min 1 (S x)) with 1 in H
+                         | [ H : context[min ?x ?y], H' : ?x <= ?y |- _ ] => rewrite Min.min_l in H by assumption
+                         | [ H : context[min ?x ?y], H' : ?y <= ?x |- _ ] => rewrite Min.min_r in H by assumption
+                         | [ H : context[min (?x - ?y) ?x] |- _ ] => rewrite Min.min_l in H by omega
+                         | [ H : context[min ?x (?x - ?y)] |- _ ] => rewrite Min.min_r in H by omega
+                         | _ => omega
+                       end.
+
+ }
+        {
+          repeat match goal with
+                   | [ H : parse_of_production _ _ [] |- _ ] => let H' := fresh in rename H into H'; dependent destruction H'
+                   | [ H : parse_of_item _ _ (Terminal _) |- _ ] => let H' := fresh in rename H into H'; dependent destruction H'
+                 end;
+            fin.
+          repeat match goal with
+                       end.
+          match goal with
+          end.
+SearchAbout min.
+          SearchAbout (_ <= 0).
+          end
+
+SearchAbout (?x - ?y) (?x <= ?y).
+SearchAbout (_ + 0).
+          Check string_bl.
+
+          admit. }
+        { clear IHls; intros.
+          repeat match goal with
+                   | [ H : parse_of_production _ _ [] |- _ ] => let H' := fresh in rename H into H'; dependent destruction H'
+                   | [ H : parse_of_production _ _ (_::_) |- _ ] => let H' := fresh in rename H into H'; dependent destruction H'
+                   | [ H : parse_of_item _ _ (Terminal _) |- _ ] => let H' := fresh in rename H into H'; dependent destruction H'
+                 end;
+            fin.
+          admit. }
+
+
+SearchAbout string_beq.
+          left; fin.
+          repeat match goal with
+                         | _ => intro
+                         | _ => progress subst
+                         | [ |- List.In ?x [?y] ] => left
+                         | _ => reflexivity
+                         | [ H : parse_of_production _ _ nil |- _ ] => let H' := fresh in rename H into H'; dependent destruction H'
+                         | [ H : parse_of_production _ _ (_::_) |- _ ] => let H' := fresh in rename H into H'; dependent destruction H'
+                         | [ H : parse_of_item _ _ (Terminal _) |- _ ] => let H' := fresh in rename H into H'; dependent destruction H'
+                         | [ H : parse_of_item _ _ (NonTerminal _ _) |- _ ] => let H' := fresh in rename H into H'; dependent destruction H'
+                         | _ => erewrite <- has_only_terminals_length by eassumption
+                         | [ H : _ |- _ ] => progress rewrite ?(@drop_length _ string_stringlike string_stringlike_properties), ?(@take_length _ string_stringlike string_stringlike_properties), ?substring_length, ?Nat.add_sub, ?Minus.minus_diag, ?Nat.sub_0_r, ?sub_plus in H by omega
+                         | _ => progress rewrite ?drop_length, ?take_length, ?substring_length, ?Nat.add_sub, ?Minus.minus_diag, ?Nat.sub_0_r, ?sub_plus by omega
+                         | [ H : context[(_ ~= [ _ ])%string_like] |- _ ]
+                           => apply length_singleton in H
+                         | [ |- context[min ?x (?y + ?z) - ?z] ]
+                           => rewrite <- (Nat.sub_min_distr_r x (y + z) z)
+                         | [ H : context[min ?x (?y + ?z) - ?z] |- _ ]
+                           => rewrite <- (Nat.sub_min_distr_r x (y + z) z) in H
+                         | [ H : min ?x ?y = 1 |- _ ] => is_var x; revert H; apply (Min.min_case_strong x y)
+                         | [ |- context[0 + ?x] ] => change (0 + x) with x
+                         | [ |- context[?x - S ?y] ]
+                           => not constr_eq y 0; rewrite !(Nat.sub_succ_r x y), !Minus.pred_of_minus
+                         | [ H : ?x = 1 |- context[?x] ] => rewrite H
+                         | [ H : ?x = 1, H' : context[?x] |- _ ] => rewrite H in H'
+                         | [ H : ?x <= ?y |- context[?x - ?y] ] => replace (x - y) with 0 by (clear -H; omega)
+                         | _ => omega
+                       end.
+          repeat match goal with
+                         | _ => intro
+                         | _ => reflexivity
+                         | _ => rewrite substring_substring
+                         | _ => rewrite Nat.sub_0_r
+                         | _ => rewrite substring_length
+                         | _ => rewrite Nat.add_sub
+                         | _ => rewrite <- Nat.sub_min_distr_r
+                         | _ => progress simpl
+                         | [ |- context[min ?x ?y] ]
+                           => match goal with
+                                | [ |- context[min y x] ]
+                                  => rewrite (Min.min_comm x y)
+                              end
+                         | [ |- context[min (min _ ?x) (?x - ?y)] ]
+                           => rewrite <- (Min.min_assoc _ x (x - y)), (Min.min_r x (x - y)) by omega
+                         | [ |- substring (?x + ?y) _ _ = substring (?y + ?x) _ _ ]
+                           => rewrite (Plus.plus_comm x y)
+                         | [ |- substring ?x ?y ?z = substring ?x (min ?w ?y) ?z ]
+                           => apply (@Min.min_case_strong w y)
+                         | [ H : _ |- _ ] => rewrite Min.min_assoc in H
+                         | _ => apply substring_correct4; omega
+                       end.
+                     fin.
+          left; fin.
+
+
+
+  rewrite <- H.
+
+
+      induction (Valid_nonterminals G) as [ | x xs ]; trivial; [].
+      { simpl.
+        rewrite !flatten_app, !fold_right_app.
+
+        destruct (G x) as [ | x' xs' ]; simpl.
+        { induction xs as [ | x'' xs'' ]; simpl; trivial; [].
+          { rewrite !flatten_app, !fold_right_app.
+      apply p.
+match goal with
+
+match goal with
+        | [ H : computes_to (fold_right _ _ _) ?v |- _ ] => clear -H; generalize dependent v
+      end.
+
+      induction (Valid_nonterminals G) as [ | x xs IHnt ]; simpl in *.
+      { simpl in *; intros; destruct_head ex; destruct_head and; destruct_head False. }
+      { intro v1.
+        rewrite flatten_app, fold_right_app.
+        intros H0 n H1 H2 H3 [nt [prefix [ [H4|H4] H4'] ] ].
+        { subst.
+        specialize (fun v1 H0 H4 => IHnt v1 H0 n H1 H2 H3 (ex_intro _ nt (ex_intro _ prefix H4))); simpl in *.
+        induction (G nt).
+        { intros; destruct_head ex; destruct_head and; destruct_head or; subst;
+          repeat match goal with
+                   | [ H : _ |- _ ] => not constr_eq H HG; rewrite HG in H
+                   | _ => progress simpl in *
+                   | [ H : False |- _ ] => destruct H
+                 end. }
+        { destruct_head and; destruct_head or; subst.
+        induction (G nt)
+Goal forall P Q, (P \/ ~P) -> (((P -> Q) -> P) -> P).
+  intros P Q [p|np] pq.
+  exact p.
+  apply pq.
+  intro
+  destruce
+
+intros; destruct_head ex; destruct_head and; destruct_head or; subst.
+
+        { apply IHnt; clear IHnt.
+
+repeat match goal with
+                 | [ H : _ |- _ ] => rewrite flatten_app in H
+                 | [ H : _ |- _ ] => rewrite fold_right_app in H
+               end.
+        SearchAbout fold_right app.
+rewrite flatten_append in H0'.
+
+    repeat match goal with
+                 | _ => progress simpl in *
+                 | _ => progress computes_to_inv
+                 | _ => progress subst
+                 (*| [ H : context[match ?x with _ => _ end] |- _ ] => (is_var x; destruct x)
+                 | [ |- context[match ?x with _ => _ end] ] => (is_var x; destruct x)
+                 | [ H : context[match ?x with _ => _ end] |- _ ] => destruct x eqn:?*)
+                 | [ |- computes_to (Bind _ _) _ ]
+                   => refine ((fun H0 H1 => BindComputes _ _ _ _ H1 H0) _ _)
+                 | [ |- computes_to (Return ?x) ?y ]
+                   => cut (x = y);
+                 [ let H := fresh in intro H; try rewrite H; eapply ReturnComputes | ]
+                 | [ |- computes_to (Pick _) _ ]
+                   => eapply PickComputes
+                 | _ => reflexivity
+                 | _ => assumption
+               end.
+
+
+      ).
+  Defined.
+
+  (*Lemma AllTheSteps
+  : Sharpened (string_spec G).
+    eapply SharpenStep.
+    apply FirstStep.
+
+    (*hone representation using
+         (fun r_o r_n =>
+                    substring (fst (snd r_n)) (snd (snd r_n)) (fst r_n) = r_o).
+    hone constructor "new".
+    {
+      simplify with monad laws.
+      refine pick val (d, (0, String.length d)).
+      subst H; higher_order_reflexivity.
+      simpl.
+      finish honing. *)
+
+  Admitted.
+*)
+End IndexedImpl.
+
+
+
+(** * Reflective helpers for simply-typed interface of the parser *)
+Require Import Coq.Lists.List Coq.Strings.String.
+Require Import Coq.Arith.Lt.
+Require Import ADTSynthesis.Parsers.ContextFreeGrammar.
+Require Import ADTSynthesis.Parsers.ContextFreeGrammarProperties.
+Require Import ADTSynthesis.Parsers.StringLike.Core.
+Require Import ADTSynthesis.Parsers.ParserInterface.
+Require Import ADTSynthesis.Parsers.ParserADTSpecification.
+Require Import ADTSynthesis.Parsers.StringLike.Properties.
+Require Import ADTSynthesis.Parsers.StringLike.String.
+Require Import ADTNotation.BuildADT ADTNotation.BuildADTSig.
+Require Import ADT.ComputationalADT.
+Require Import ADTSynthesis.ADTRefinement.
+Require Import ADTSynthesis.Common.StringBound ADTSynthesis.Common.ilist.
+Require Import ADTRefinement.BuildADTRefinements.HoneRepresentation.
+Require Import ADTSynthesis.Common.IterateBoundedIndex.
+Require Import ADTSynthesis.Computation.Core ADTSynthesis.Computation.ApplyMonad ADTSynthesis.Computation.Monad ADTSynthesis.Computation.SetoidMorphisms.
+Require Import ADTSynthesis.Common.SetoidInstances.
+
+Set Implicit Arguments.
+
+Section interface.
+  Context (G : grammar Ascii.ascii).
+
+  Local Notation string_of_indexed s :=
+    (substring (fst (snd s)) (snd (snd s)) (fst s))
+      (only parsing).
+  Local Notation ilength s :=
+    (min (String.length (fst s) - fst (snd s)) (snd (snd s)))
+      (only parsing).
+
+
+
+Set Implicit Arguments.
+
+Local Open Scope list_scope.
+Local Open Scope ADTSig_scope.
+Local Open Scope ADT_scope.
+Local Open Scope string_scope.
+
+Section helpers.
+  Section generic.
+    Context {Char : Type}.
+
+    Fixpoint has_only_terminals (its : production Char)
+    : bool
+      := match its with
+           | nil => true
+           | (Terminal _)::xs => has_only_terminals xs
+           | (NonTerminal _)::_ => false
+         end.
+  End generic.
+
+  Section generic_string.
+    Context {Char} {HSL : StringLike Char} {HLSP : StringLikeProperties Char} (G : grammar Char).
+
+    Lemma has_only_terminals_length {its str}
+          (H0 : @has_only_terminals _ its)
+          (H1 : parse_of_production G str its)
+    : length str = List.length its.
+    Proof.
+      induction H1 as [ | ? ? ? ? pit pits IH ]; simpl in *; trivial.
+      rewrite drop_length in IH.
+      dependent destruction pit.
+      { match goal with
+          | [ H : context[(_ ~= [ _ ])%string_like] |- _ ]
+            => apply length_singleton in H
+        end.
+        rewrite <- IH by assumption; clear IH.
+        repeat match goal with
+                 | _ => intro
+                 | [ H : context[length (take _ _)] |- _ ] => rewrite take_length in H
+                 | [ H : context[length (drop _ _)] |- _ ] => rewrite drop_length in H
+                 | [ H : min ?x ?y = 1 |- _ ] => is_var x; destruct x
+                 | [ H : min (S ?x) ?y = 1 |- _ ] => is_var x; destruct x
+                 | [ H : min (S (S ?x)) ?y = 1 |- _ ] => revert H; apply (Min.min_case_strong (S (S x)) y)
+                 | [ H : context[min _ 0] |- _ ] => rewrite Min.min_0_r in H
+                 | [ H : context[min 0 _] |- _ ] => rewrite Min.min_0_l in H
+                 | [ H : 0 = 1 |- _ ] => exfalso; clear -H; discriminate
+                 | [ H : S (S _) = 1 |- _ ] => exfalso; clear -H; discriminate
+                 | [ H : ?x = 1, H' : context[?x] |- _ ] => rewrite H in H'
+                 | [ H : ?x = 1 |- context[?x] ] => rewrite H
+                 | [ H : min ?x ?y = 1 |- _ ] => revert H; apply (Min.min_case_strong x y)
+                 | _ => omega
+               end. }
+      { exfalso.
+        unfold is_true in *.
+        discriminate. }
+    Qed.
+  End generic_string.
+End helpers.
+
+Section IndexedImpl.
+  Context (G : grammar Ascii.ascii).
+
+  Local Notation T := (String.string * (nat * nat))%type (only parsing).
+
+  Local Notation string_of_indexed s :=
+    (substring (fst (snd s)) (snd (snd s)) (fst s))
+      (only parsing).
+  Local Notation ilength s :=
+    (min (String.length (fst s) - fst (snd s)) (snd (snd s)))
+      (only parsing).
+
+  (** Reference implementation of a [String] that can be split; has a [string], and a start index, and a length *)
+  (** TODO: should we replace
+
+       [string_dec (string_of_indexed s) (String.String ch "") : bool]
+
+      with something fancier and maybe more efficient, like
+
+        [((Nat.eq_dec (min (String.length base - fst s) (snd s)) 1) &&
+  (option_dec Ascii.ascii_dec (String.get (fst s) base) (Some
+  ch)))%bool] *)
+
+  Definition indexed_spec : ADT (string_rep Ascii.ascii) := ADTRep T {
+    Def Constructor "new"(s : String.string) : rep :=
+      ret (s, (0, String.length s)),
+
+    Def Method "to_string"(s : rep, x : unit) : String.string :=
+      ret (s, string_of_indexed s),
+
+    Def Method "is_char"(s : rep, ch : Ascii.ascii) : bool  :=
+      ret (s, string_beq (string_of_indexed s) (String.String ch "")),
+
+    Def Method "length"(s : rep, x : unit) : nat :=
+      ret (s, ilength s),
+
+    Def Method "take"(s : rep, n : nat) : unit :=
+      ret ((fst s, (fst (snd s), min (snd (snd s)) n)), tt),
+
+    Def Method "drop"(s : rep, n : nat) : unit :=
+      ret ((fst s, (fst (snd s) + n, snd (snd s) - n)), tt),
+
+    Def Method "splits"(s : rep, p : item Ascii.ascii * production Ascii.ascii) : list nat :=
+      fallback_ls <- { ls : list nat
+                     | match fst p with
+                         | Terminal _
+                           => True
+                         | NonTerminal _
+                           => if has_only_terminals (snd p)
+                              then True
+                              else split_list_is_complete G (string_of_indexed s) (fst p) (snd p) ls
+                       end };
+      let ls := (match snd p, fst p with
+                   | nil, _
+                     => [ilength s]
+                   | _::_, Terminal _
+                     => [1]
+                   | _::_, NonTerminal _
+                     => if has_only_terminals (snd p)
+                        then [ilength s - List.length (snd p)]
+                        else fallback_ls
+                 end) in
+      ret (s, ls)
+  }.
+
+  Lemma FirstStep
+  : refineADT (string_spec G) indexed_spec.
+  Proof.
+    econstructor 1 with (AbsR := (fun r_o r_n =>
+                                    substring (fst (snd r_n)) (snd (snd r_n)) (fst r_n) = r_o));
+    abstract (
+        eapply Iterate_Ensemble_BoundedIndex_equiv;
+        simpl; intuition; intros; try simplify with monad laws;
+        repeat intro; computes_to_inv; subst; simpl;
+        repeat match goal with
+                 | _ => progress simpl in *
+                 | _ => progress computes_to_inv
+                 | _ => progress subst
+                 | [ H : context[match ?x with _ => _ end] |- _ ] => (is_var x; destruct x)
+                 | [ |- context[match ?x with _ => _ end] ] => (is_var x; destruct x)
+                 | [ H : context[match ?x with _ => _ end] |- _ ] => destruct x eqn:?
+                 | [ |- computes_to (Bind _ _) _ ]
+                   => refine ((fun H0 H1 => BindComputes _ _ _ _ H1 H0) _ _)
+                 | [ |- computes_to (Return ?x) ?y ]
+                   => cut (x = y);
+                 [ let H := fresh in intro H; try rewrite H; eapply ReturnComputes | ]
+                 | [ |- computes_to (Pick _) _ ]
+                   => eapply PickComputes
+                 | _ => reflexivity
+                 | _ => assumption
+               end;
+        try solve [ rewrite substring_correct3'; reflexivity
+                  | repeat match goal with
+                             | _ => intro
+                             | _ => reflexivity
+                             | _ => rewrite substring_substring
+                             | _ => rewrite Nat.sub_0_r
+                             | _ => rewrite substring_length
+                             | _ => rewrite Nat.add_sub
+                             | _ => rewrite <- Nat.sub_min_distr_r
+                             | _ => progress simpl
+                             | [ |- context[min ?x ?y] ]
+                               => match goal with
+                                    | [ |- context[min y x] ]
+                                      => rewrite (Min.min_comm x y)
+                                  end
+                             | [ |- context[min (min _ ?x) (?x - ?y)] ]
+                               => rewrite <- (Min.min_assoc _ x (x - y)), (Min.min_r x (x - y)) by omega
+                             | [ |- substring (?x + ?y) _ _ = substring (?y + ?x) _ _ ]
+                               => rewrite (Plus.plus_comm x y)
+                             | [ |- substring ?x ?y ?z = substring ?x (min ?w ?y) ?z ]
+                               => apply (@Min.min_case_strong w y)
+                             | [ H : _ |- _ ] => rewrite Min.min_assoc in H
+                             | _ => apply substring_correct4; omega
+                           end
+                  | repeat match goal with
+                             | _ => intro
+                             | _ => progress subst
+                             | [ |- List.In ?x [?y] ] => left
+                             | _ => reflexivity
+                             | [ H : parse_of_production _ _ nil |- _ ] => let H' := fresh in rename H into H'; dependent destruction H'
+                             | [ H : parse_of_production _ _ (_::_) |- _ ] => let H' := fresh in rename H into H'; dependent destruction H'
+                             | [ H : parse_of_item _ _ (Terminal _) |- _ ] => let H' := fresh in rename H into H'; dependent destruction H'
+                             | [ H : parse_of_item _ _ (NonTerminal _ _) |- _ ] => let H' := fresh in rename H into H'; dependent destruction H'
+                             | _ => erewrite <- has_only_terminals_length by eassumption
+                             | [ H : _ |- _ ] => progress rewrite ?(@drop_length _ string_stringlike string_stringlike_properties), ?(@take_length _ string_stringlike string_stringlike_properties), ?substring_length, ?Nat.add_sub, ?Minus.minus_diag, ?Nat.sub_0_r, ?sub_plus in H by omega
+                             | _ => progress rewrite ?drop_length, ?take_length, ?substring_length, ?Nat.add_sub, ?Minus.minus_diag, ?Nat.sub_0_r, ?sub_plus by omega
+                             | [ H : context[(_ ~= [ _ ])%string_like] |- _ ]
+                               => apply length_singleton in H
+                             | [ |- context[min ?x (?y + ?z) - ?z] ]
+                               => rewrite <- (Nat.sub_min_distr_r x (y + z) z)
+                             | [ H : context[min ?x (?y + ?z) - ?z] |- _ ]
+                               => rewrite <- (Nat.sub_min_distr_r x (y + z) z) in H
+                             | [ H : min ?x ?y = 1 |- _ ] => is_var x; revert H; apply (Min.min_case_strong x y)
+                             | [ |- context[0 + ?x] ] => change (0 + x) with x
+                             | [ |- context[?x - S ?y] ]
+                               => not constr_eq y 0; rewrite !(Nat.sub_succ_r x y), !Minus.pred_of_minus
+                             | [ H : ?x = 1 |- context[?x] ] => rewrite H
+                             | [ H : ?x = 1, H' : context[?x] |- _ ] => rewrite H in H'
+                             | [ H : ?x <= ?y |- context[?x - ?y] ] => replace (x - y) with 0 by (clear -H; omega)
+                             | _ => omega
+                           end ]
+      ).
+  Defined.
+
+  (*Lemma AllTheSteps
+  : Sharpened (string_spec G).
+    eapply SharpenStep.
+    apply FirstStep.
+
+    (*hone representation using
+         (fun r_o r_n =>
+                    substring (fst (snd r_n)) (snd (snd r_n)) (fst r_n) = r_o).
+    hone constructor "new".
+    {
+      simplify with monad laws.
+      refine pick val (d, (0, String.length d)).
+      subst H; higher_order_reflexivity.
+      simpl.
+      finish honing. *)
+
+  Admitted.
+*)
+End IndexedImpl.
+
 
   Lemma step_expanded_fallback_list {s p} dummy
   : refine (fallback_ls <- {ls : list nat |
@@ -99,10 +996,293 @@ Section interface.
   Proof.
     unfold expanded_fallback_list, forall_reachable_productions, split_list_is_complete, production_is_reachable.
     generalize (Valid_nonterminals G).
-    intro ls; revert p; induction ls.
+    match goal with
+      | [ |- context[match snd p with nil => ?x | _ => _ end] ]
+        => let H := fresh "nil_case" in generalize x; intro H
+    end.
+    generalize (has_only_terminals (snd p)); intro test.
+    generalize [1]; intro one_list.
+    intro ls.
+    match goal with
+      | [ |- context[if test then [?x - _] else _] ]
+        => not constr_eq x True; let H := fresh "then_case" in generalize x; intro H
+    end.
+    induction ls.
     { simpl.
       repeat intro; computes_to_inv; subst.
-      destruct (fst p); simpl.
+      destruct (fst p), (snd p); simpl;
+      repeat match goal with
+               | [ |- computes_to (Bind _ _) _ ]
+                 => refine ((fun H0 H1 => BindComputes _ _ _ _ H1 H0) _ _)
+               | [ |- computes_to (Return _) _ ]
+                 => apply ReturnComputes
+               | [ |- computes_to (Pick _) _ ]
+                 => apply PickComputes
+               | _ => solve [ trivial ]
+               | _ => intro
+               | _ => progress destruct_head ex
+               | _ => progress destruct_head and
+               | _ => progress destruct_head False
+               | [ |- if ?e then _ else _ ] => case_eq e
+             end. }
+    { simpl.
+      setoid_rewrite flatten_app.
+      setoid_rewrite fold_right_app.
+      lazymatch goal with
+        | [ |- refine _ (ls <- fold_right ?f ?x ?k; ret (?s, ls)) ]
+          => transitivity (ls <- fold_right f (lss <- (ls <- x; ret (s, ls)); ret (snd lss)) k; ret (s, ls))%comp;
+            [
+            | setoid_rewrite refineEquiv_bind_bind;
+              setoid_rewrite refineEquiv_bind_unit; simpl;
+              setoid_rewrite refineEquiv_unit_bind;
+              reflexivity ]
+      end.
+      setoid_rewrite <- IHls; clear IHls.
+      setoid_rewrite refineEquiv_bind_bind.
+      setoid_rewrite refineEquiv_bind_unit; simpl.
+      let LHS := match goal with |- refine ?LHS ?RHS => constr:LHS end in
+      lazymatch LHS with
+        | context G0[exists (nt : string) (prefix : list ?A),
+                      (?a = nt \/ In nt ?ls) /\
+                      In (prefix ++ ?rest) (Lookup ?G nt)]
+          => let H := fresh in
+             assert (H : (exists nt prefix, (a = nt \/ In nt ls) /\ In (prefix ++ rest) (Lookup G nt)) <-> (exists prefix, In (prefix ++ rest) (Lookup G a)) \/ (exists nt prefix, In nt ls /\ In (prefix ++ rest) (Lookup G nt)))
+             by (split; intros; repeat (destruct_head ex || destruct_head or);
+                   intuition (subst; eauto));
+             let G' := context G0[(exists prefix, In (prefix ++ rest) (Lookup G a)) \/ (exists nt prefix, In nt ls /\ In (prefix ++ rest) (Lookup G nt))] in
+             transitivity G'
+      end.
+      { apply refine_bind_Proper; [ | reflexivity ].
+        apply refine_flip_impl_Pick_Proper.
+        destruct (fst p).
+        typeclasses eauto.
+        destruct test.
+        typeclasses eauto.
+        intro.
+        intros ?.
+
+Goal forall {A B} (H : A <-> B), forall n : nat, n = n -> B.
+  intros A B H.
+  setoid_rewrite <- H.
+        setoid_rewrite H.
+        typeclasses eauto.
+        intro.
+        unfold flip.
+        SearchAbout impl.
+        destruct (fst p); trivial.
+intros ??.
+
+        destruct (fst p).
+        setoid_rewrite H.
+               by (split; intros; repeat (destruct_head ex || destruct_head or);
+                   intuition (subst; eauto));
+               let P := fresh in
+               set (P := exists nt prefix, (a = nt \/ In nt ls) /\ In (prefix ++ rest) (Lookup G nt)) in *
+      end.
+      setoid_rewrite H.
+
+      Typeclasses eauto := debug.
+      setoid_rewrite H.
+      {
+
+
+      intuition.
+ tauto.
+      repeat intro;
+        computes_to_inv; subst.
+      computes_to_inv.
+              setoid_rewrite refineEquiv_unit_bind;
+
+      Typeclasses eauto := debug.
+      Focus 2.
+
+
+      pose proof (_ : (Proper (refine ==> _ ==> _)
+   (fold_right
+      (fun (p0 : production Ascii.ascii) (else_case : Comp (list nat)) =>
+       if production_beq ascii_beq p0 (fst p :: snd p)
+       then
+        match p0 with
+        | [] => ret dummy
+        | [Terminal _] => ret nil_case
+        | Terminal _ :: _ :: _ => ret one_list
+        | [NonTerminal nt] => ret nil_case
+        | NonTerminal nt :: (_ :: _) as p' =>
+            if has_only_terminals p'
+            then ret [then_case - Datatypes.length p']
+            else
+             {splits : list nat |
+             forall n : nat,
+             n <= String.length (fst s) ->
+             parse_of_item G (substring 0 n (fst s)) (NonTerminal nt) ->
+             parse_of_production G
+               (substring n (String.length (fst s)) (fst s)) p' ->
+             In n splits}%comp
+        end
+       else else_case)))).
+            Typeclasses eauto := debug.
+            Timeout 1 pose proof (fun A => _ : Proper (_ ==> refine ==> impl) (@refine A)).
+
+(Proper (refine ==> flip impl)
+   (refine
+      (fallback_ls <- {ls0 : list nat |
+                      match fst p with
+                      | Terminal _ => True
+                      | NonTerminal _ =>
+                          if test
+                          then True
+                          else
+                           forall n : nat,
+                           n <=
+                           String.length
+                             (substring (fst (snd s)) (snd (snd s)) (fst s)) ->
+                           parse_of_item G
+                             (substring 0 n
+                                (substring (fst (snd s))
+                                   (snd (snd s)) (fst s)))
+                             (fst p) ->
+                           parse_of_production G
+                             (substring n
+                                (String.length
+                                   (substring (fst (snd s))
+                                      (snd (snd s))
+                                      (fst s)))
+                                (substring (fst (snd s))
+                                   (snd (snd s)) (fst s)))
+                             (snd p) ->
+                           (exists
+                              (nt : string) (prefix :
+                                             list (item Ascii.ascii)),
+                              (a = nt \/ In nt ls) /\
+                              In (prefix ++ fst p :: snd p) (G nt)) ->
+                           In n ls0
+                      end};
+       ret
+         (s,
+         match snd p with
+         | [] => nil_case
+         | _ :: _ =>
+             match fst p with
+             | Terminal _ => one_list
+             | NonTerminal _ =>
+                 if test
+                 then [then_case - Datatypes.length (snd p)]
+                 else fallback_ls
+             end
+         end))))
+
+      Focus 2.
+      pose proof (_ : (Proper (refineEquiv ==> _ ==> _)
+   (fold_right
+      (fun (p0 : production Ascii.ascii) (else_case : Comp (list nat)) =>
+       if production_beq ascii_beq p0 (fst p :: snd p)
+       then
+        match p0 with
+        | [] => ret dummy
+        | [Terminal _] => ret nil_case
+        | Terminal _ :: _ :: _ => ret one_list
+        | [NonTerminal nt] => ret nil_case
+        | NonTerminal nt :: (_ :: _) as p' =>
+            if has_only_terminals p'
+            then ret [then_case - Datatypes.length p']
+            else
+             {splits : list nat |
+             forall n : nat,
+             n <= String.length (fst s) ->
+             parse_of_item G (substring 0 n (fst s)) (NonTerminal nt) ->
+             parse_of_production G
+               (substring n (String.length (fst s)) (fst s)) p' ->
+             In n splits}%comp
+        end
+       else else_case)))).
+      pose proof (_ : (ProperProxy eq (flatten (map tails (G a))))).
+      setoid_rewrite refineEquiv_bind_bind.
+
+
+
+      Check (_ : (Proper
+                    (pointwise_relation (production Ascii.ascii)
+      (refineEquiv ==> refineEquiv)%signature)
+   (fun (p0 : production Ascii.ascii) (else_case : Comp (list nat)) =>
+    if production_beq ascii_beq p0 (fst p :: snd p)
+    then
+     match p0 with
+     | [] => ret dummy
+     | [Terminal _] => ret nil_case
+     | Terminal _ :: _ :: _ => ret one_list
+     | [NonTerminal nt] => ret nil_case
+     | NonTerminal nt :: (_ :: _) as p' =>
+         if has_only_terminals p'
+         then ret [then_case - Datatypes.length p']
+         else
+          {splits : list nat |
+          forall n : nat,
+          n <= String.length (fst s) ->
+          parse_of_item G (substring 0 n (fst s)) (NonTerminal nt) ->
+          parse_of_production G (substring n (String.length (fst s)) (fst s))
+            p' -> In n splits}%comp
+     end
+    else else_case))).
+
+      Focus 2.
+      intro.
+      match goal with
+        | [ |- ?R ?f ?f ] => change (Proper R f)
+      end.
+      exact _.
+
+
+      .
+      match goal with
+        | [ |- refine (u <- ?x; u' <- ret (@?f u); ret (@?g u')) _ ]
+          => transitivity (u <- x; ret (g (f (u))))%comp;
+            [ apply refine_bind_Proper;
+              [ reflexivity | ]
+            | ]
+      end.
+      intro; simpl.
+
+      rewrite <- refine_unit_bind'.
+      3:rewrite refineEquiv_bind_bind.
+      Focus 2.
+      { asse
+
+Lemma refineEquiv_bind_bind_ret {A B C} (c1 : Comp A) (f1 : A -> Comp B) (f2 : B -> Comp C)
+: refineEquiv (b <- (a <- c1; f1 a); f2 b) (a <- c1; b <- f1 a; f2 b).
+Proof.
+  split; repeat intro; computes_to_inv;
+  repeat repeat (eassumption || refine ((fun H0 H1 => BindComputes _ _ _ _ H1 H0) _ _)).
+Qed.
+Lemma refine_bind_bind_ret {A B C} (c1 : Comp A) (f1 : A -> Comp B) (f2 : B -> Comp C)
+: refine (b <- (a <- c1; f1 a); f2 b) (a <- c1; b <- f1 a; f2 b).
+Proof.
+  apply refineEquiv_bind_bind_ret.
+Qed.
+Lemma refine_bind_bind_ret' {A B C} (c1 : Comp A) (f1 : A -> Comp B) (f2 : B -> Comp C)
+: refine (a <- c1; b <- f1 a; f2 b) (b <- (a <- c1; f1 a); f2 b).
+Proof.
+  apply refineEquiv_bind_bind_ret.
+Qed.
+Focus 2.
+SearchAbout refine Bind.
+apply refine_fold_right.
+SearchAbout refine fold_right.
+apply fold_right_refine_Proper.
+setoid_rewrite refine_bind_bind_ret.
+
+      SearchAbout (_ <- _ (_ <- _; ret _); _)%comp.
+      Focus 2.
+      SearchAbout refine Bind.
+      simplify with setoid-y monad laws.
+      end.
+
+setoid_rewrite IHls.
+      match goal with
+        | [ |
+      SearchAbout fold_right app.
+  SearchAbout (_ ++ _ ++ _).
+      SearchAbout flatten1 append.
+      match goal with
       {
     intro ls; induction ls
     simplify with monad laws.
@@ -174,3 +1354,6 @@ Section interface.
                              -> has_parse str = true
     }.
 End interface.
+
+
+Global Arguments forall_reachable_productions / .
